Algorithm/Data/Classes/IndexedMinHeap.lean
@@ -1,0 +1,45 @@
+/-
+Copyright (c) 2023 Yuyang Zhao. All rights reserved.
+Released under Apache 2.0 license as described in the file LICENSE.
+Authors: Yuyang Zhao
+-/
+import Algorithm.Data.Classes.AssocArray
+import Mathlib.Data.Finset.Lattice
+import Mathlib.Data.Prod.Lex
+
+class IndexedMinHeap (H : Type*) (ι : outParam Type*) [DecidableEq ι]
+    (α : outParam Type*) [LinearOrder α] extends AssocArray H ι (WithTop α) where
+  minIdx : H → ι
+  get_minIdx_le h (i : ι) : h[minIdx h] ≤ h[i]
+
+namespace ArrayVector
+variable {α : Type*} [LinearOrder α] {n : ℕ} [NeZero n]
+
+def minAux (a : ArrayVector (WithTop α) n) : Lex (WithTop α × Fin n) :=
+  (⊤ : Finset (Fin n)).inf' ⟨0, Finset.mem_univ 0⟩ (fun i ↦ toLex (a[i], i))
+
+def minIdx (a : ArrayVector (WithTop α) n) : Fin n :=
+  a.minAux.2
+
+def minIdx_spec (a : ArrayVector (WithTop α) n) (i : Fin n) :
+    a[a.minIdx] < a[i] ∨ a[a.minIdx] = a[i] ∧ a.minIdx ≤ i := by
+  have : a.minAux.1 = a[a.minIdx]
+  · unfold minIdx minAux
+    obtain ⟨i, -, h⟩ := (⊤ : Finset (Fin n)).exists_mem_eq_inf'
+      ⟨0, Finset.mem_univ 0⟩ (fun i ↦ toLex (a[i], i))
+    rw [Prod.eq_iff_fst_eq_snd_eq] at h
+    obtain ⟨h : _ = a[i], rfl : _ = i⟩ := h
+    exact h
+  rw [← this]
+  apply (Prod.Lex.le_iff _ (a[i], i)).mp
+  exact Finset.inf'_le _ (Finset.mem_univ _)
+
+def minIdx_le (a : ArrayVector (WithTop α) n) (i : Fin n) :
+    a[a.minIdx] ≤ a[i] :=
+  (a.minIdx_spec i).elim LT.lt.le (fun ⟨h, _⟩ ↦ h.le)
+
+instance [NeZero n] : IndexedMinHeap (ArrayVector (WithTop α) n) (Fin n) α where
+  minIdx a := ((⊤ : Finset (Fin n)).inf' ⟨0, Finset.mem_univ 0⟩ (fun i ↦ toLex (a[i], i))).2
+  get_minIdx_le a i := a.minIdx_le i
+
+end ArrayVector
